# Problem 1

## Derivation of Kepler's Third Law

### Step 1: Gravitational and Centripetal Forces

Newton's Law of Gravitation:

$$
F_g = \frac{G M m}{r^2}
$$

Centripetal force for circular motion:  

$$
F_c = m \frac{v^2}{r}
$$

Equating $$F_g = F_c$$ :

$$
\frac{G M m}{r^2} = m \frac{v^2}{r}
$$

Canceling $$m$$ :

$$
\frac{G M}{r^2} = \frac{v^2}{r}
$$

Multiplying by $$r$$ :

$$
v^2 = \frac{G M}{r}
$$


### Step 2: Expressing in Terms of Orbital Period  

Using  $$v = \frac{2\pi r}{T}$$ :
$$\left( \frac{2\pi r}{T} \right)^2 = \frac{G M}{r}$$
$$
\frac{4\pi^2 r^2}{T^2} = \frac{G M}{r}
$$

Multiplying by $$r$$ : 

$$
4\pi^2 r^3 = G M T^2
$$

### Step 3: Final Relation  

$$
T^2 = \frac{4\pi^2}{G M} r^3
$$

Thus,

$$
T^2 \propto r^3
$$

Keplerâ€™s Third Law is derived.